Move syntax to autosubst, prove congurence lemma and STS shape

theories/signatures/pi.sig
@@ -1,0 +1,30 @@
+-- I can add a preamble with -p to autosubst!!
+-- If something doesn't work: try adding scons_eta' from unscoped.v to asimpl
+-- Note: in π calculus Channels are Values (so there is just one type)
+
+proc  : Type
+Data : Type
+
+Value : Type
+Equation : Type
+
+cst : Value -> Data
+
+tt : Equation
+ff : Equation
+Inequality : Data -> Data -> Equation
+Or : Equation -> Equation -> Equation
+Not : Equation -> Equation
+
+pr_success : proc
+pr_nil : proc
+pr_rec : (bind proc in proc) -> proc
+pr_choice : proc -> proc -> proc
+pr_par : proc -> proc -> proc
+pr_output : Data  -> Data -> proc -> proc
+pr_res : (bind Data in proc) -> proc
+pr_input : Data -> (bind Data in proc) -> proc
+-- pr_res : (bind Data in proc) -> proc
+-- pr_input : Data -> (bind Data in proc) -> proc
+pr_tau : proc -> proc
+pr_if_then_else : Equation -> proc -> proc -> proc
